Add OID and tests with mbedTLS.

src/asn1/ASN1.Test.Helpers.c
@@ -1,6 +1,61 @@
 #include <string.h>
+#include <stdio.h>
+#include "mbedtls/asn1.h"
+#include "mbedtls/asn1write.h"
 
 _Bool buffer_eq (unsigned char *b1, unsigned char *b2, size_t l)
 {
   return memcmp (b1, b2, l) == 0;
+}
+
+void mbedtls_parse_INTEGER (uint8_t *buf, size_t len, size_t pos)
+{
+  uint8_t *c;
+  c = buf + pos;
+  int32_t val;
+  mbedtls_asn1_get_int (&c, buf + len, &val);
+  printf ("Parsed  : %d\n", val);
+  return;
+}
+
+void mbedtls_parse_BOOLEAN (uint8_t *buf, size_t len, size_t pos)
+{
+  uint8_t *c;
+  c = buf + pos;
+  int32_t val;
+  mbedtls_asn1_get_bool (&c, buf + len, &val);
+  printf ("Parsed  : %d\n", val);
+  return;
+}
+
+void mbedtls_parse_NULL (uint8_t *buf, size_t len, size_t pos)
+{
+  // uint8_t *c;
+  // c = buf + pos;
+  // int ret = mbedtls_asn1_get_tag (&c, buf + len, 0, MBEDTLS_ASN1_NULL);
+  // printf("Parsed len: %d", ret);
+  printf("mbedTLS does not have NULL parser. \n");
+  return;
+}
+
+void mbedtls_parse_BIT_STRING (uint8_t *buf, size_t len, size_t pos)
+{
+  uint8_t *c;
+  c = buf + pos;
+  mbedtls_asn1_bitstring bs;
+  mbedtls_asn1_get_bitstring (&c, buf + len, &bs);
+
+  printf("Parsed  : len: %ld; unused_bits: %d; s: ", bs.len, bs.unused_bits);
+  for(int i = 1; i <= bs.len; i++){
+    printf("0x%x ", bs.p[i-1]);
+  }
+  printf("\n");
+
+  return;
+}
+
+void mbedtls_parse_OCTET_STRING (uint8_t *buf, size_t len, size_t pos)
+{
+  printf("mbedTLS does not have OCTET STRING parser. \n");
+  return;
 }
