src/asn1/ASN1.Low.Value.OID.fst
@@ -1,0 +1,311 @@
+module ASN1.Low.Value.OID
+
+open ASN1.Base
+open ASN1.Spec.Value.OID
+open ASN1.Low.Base
+open LowParse.Low.Bytes
+
+open FStar.Integers
+
+module HS = FStar.HyperStack
+module HST = FStar.HyperStack.ST
+module MB = LowStar.Monotonic.Buffer
+module B = LowStar.Buffer
+module Cast = FStar.Int.Cast
+
+module B32 = FStar.Bytes
+
+module IB = LowStar.ImmutableBuffer
+module CB = LowStar.ConstBuffer
+
+module G = FStar.Ghost
+
+open IB
+
+// let test (b:ibuffer int) (s:G.erased (Seq.seq int))
+// : Lemma
+//   (requires witnessed b (cpred (G.reveal s)))
+//   (ensures witnessed b (seq_eq s))
+// = assert (0 + v (len b) <= length b);
+//   assert (mgsub (immutable_preorder int) b 0ul (len b) == b);
+//   witnessed_functorial b b 0ul (len b) (cpred (G.reveal s)) (seq_eq (s))
+
+let test
+  (len: size_t)
+  (seq: lbytes (v len))
+  (ib: IB.libuffer byte (v len) seq {IB.recallable ib /\ IB.frameOf ib == HS.root} )
+: HST.St (unit)
+= IB.recall ib;
+  IB.recall_contents ib seq;
+  let x = 1 in
+()
+
+(* FIXME: Notes about `IB` and Ghost seq:
+   NOTE: `IB.cpred` vs `IB.seq_eq`, `IB.recall_contents` vs `IB.recall_value`
+   We may want to use the following `oid_seq` to represent a
+   immutable buffer, but now the `IB` library is not universally
+   using ghost seq, because HACL* is dependent on the legacy `IB`
+   which is using (witnessing, recalling over) (total) seq. The
+   allocation function `IB.igcmalloc_of_list` is one of those
+   blocked by HACL*.
+*)
+noeq
+type oid_buffer_t = {
+  oid_len: asn1_value_int32_of_type OID;
+  oid_seq: G.erased (lbytes (v oid_len));
+  oid_buf: ib: IB.libuffer byte (v oid_len) (G.reveal oid_seq) {
+           B.frameOf ib == HS.root /\
+           B.recallable ib
+  }
+}
+
+let oid_RIOT_as_buffer                     = IB.igcmalloc_of_list HS.root oid_RIOT
+let oid_AT_CN_as_buffer                    = IB.igcmalloc_of_list HS.root oid_AT_CN
+let oid_AT_COUNTRY_as_buffer               = IB.igcmalloc_of_list HS.root oid_AT_COUNTRY
+let oid_AT_ORGANIZATION_as_buffer          = IB.igcmalloc_of_list HS.root oid_AT_ORGANIZATION
+let oid_CLIENT_AUTH_as_buffer              = IB.igcmalloc_of_list HS.root oid_CLIENT_AUTH
+let oid_AUTHORITY_KEY_IDENTIFIER_as_buffer = IB.igcmalloc_of_list HS.root oid_AUTHORITY_KEY_IDENTIFIER
+let oid_KEY_USAGE_as_buffer                = IB.igcmalloc_of_list HS.root oid_KEY_USAGE
+let oid_EXTENDED_KEY_USAGE_as_buffer       = IB.igcmalloc_of_list HS.root oid_EXTENDED_KEY_USAGE
+let oid_BASIC_CONSTRAINTS_as_buffer        = IB.igcmalloc_of_list HS.root oid_BASIC_CONSTRAINTS
+
+// let oid_DIGEST_ALG_SHA224_as_buffer: oid_buffer_t
+// = { oid_len = 9ul;
+//     oid_seq = G.hide (Seq.createL oid_DIGEST_ALG_SHA224);
+//     oid_buf = IB.igcmalloc_of_list HS.root oid_DIGEST_ALG_SHA224 }
+let oid_DIGEST_ALG_SHA224_as_buffer
+= IB.igcmalloc_of_list HS.root oid_DIGEST_ALG_SHA224
+
+// let oid_DIGEST_ALG_SHA256_as_buffer: oid_buffer_t
+// = { oid_len = 9ul;
+//     oid_seq = G.hide (Seq.createL oid_DIGEST_ALG_SHA256);
+//     oid_buf = IB.igcmalloc_of_list HS.root oid_DIGEST_ALG_SHA256 }
+let oid_DIGEST_ALG_SHA256_as_buffer
+= IB.igcmalloc_of_list HS.root oid_DIGEST_ALG_SHA256
+
+// let oid_DIGEST_ALG_SHA384_as_buffer: oid_buffer_t
+// = { oid_len = 9ul;
+//     oid_seq = G.hide (Seq.createL oid_DIGEST_ALG_SHA384);
+//     oid_buf = IB.igcmalloc_of_list HS.root oid_DIGEST_ALG_SHA384 }
+let oid_DIGEST_ALG_SHA384_as_buffer
+= IB.igcmalloc_of_list HS.root oid_DIGEST_ALG_SHA384
+
+// let oid_DIGEST_ALG_SHA512_as_buffer: oid_buffer_t
+// = { oid_len = 9ul;
+//     oid_seq = G.hide (Seq.createL oid_DIGEST_ALG_SHA512);
+//     oid_buf = IB.igcmalloc_of_list HS.root oid_DIGEST_ALG_SHA512 }
+let oid_DIGEST_ALG_SHA512_as_buffer
+= IB.igcmalloc_of_list HS.root oid_DIGEST_ALG_SHA512
+
+(* NOTE: We may remove this if we are not implementing the parser. *)
+noextract
+let list_of_oid_buffers
+= [ oid_RIOT_as_buffer;
+    oid_AT_CN_as_buffer;
+    oid_AT_COUNTRY_as_buffer;
+    oid_AT_ORGANIZATION_as_buffer;
+    oid_CLIENT_AUTH_as_buffer;
+    oid_AUTHORITY_KEY_IDENTIFIER_as_buffer;
+    oid_KEY_USAGE_as_buffer;
+    oid_EXTENDED_KEY_USAGE_as_buffer;
+    oid_BASIC_CONSTRAINTS_as_buffer;
+    oid_DIGEST_ALG_SHA224_as_buffer;
+    oid_DIGEST_ALG_SHA256_as_buffer;
+    oid_DIGEST_ALG_SHA384_as_buffer;
+    oid_DIGEST_ALG_SHA512_as_buffer
+]
+let known_oids_as_buffer = IB.igcmalloc_of_list HS.root list_of_oid_buffers
+
+
+(* FIXME: A workaround
+   To not extract any (total) seq, we split the `oid_buffer_t` into three
+   functions, all of them take an `oid: oid_t`, returns the corresponding
+   len, (total) seq and ibuffer. The (total) seq will be only used in the
+   `IB.recall_contents` lemma, and the function returns the (total) seq
+   will be marded as `noextract`.
+*)
+
+let oid_buffer_of_oid
+  (oid: oid_t)
+= match oid with
+  | OID_RIOT                     -> oid_RIOT_as_buffer
+  | OID_AT_CN                    -> oid_AT_CN_as_buffer
+  | OID_AT_COUNTRY               -> oid_AT_COUNTRY_as_buffer
+  | OID_AT_ORGANIZATION          -> oid_AT_ORGANIZATION_as_buffer
+  | OID_CLIENT_AUTH              -> oid_CLIENT_AUTH_as_buffer
+  | OID_AUTHORITY_KEY_IDENTIFIER -> oid_AUTHORITY_KEY_IDENTIFIER_as_buffer
+  | OID_KEY_USAGE                -> oid_KEY_USAGE_as_buffer
+  | OID_EXTENDED_KEY_USAGE       -> oid_EXTENDED_KEY_USAGE_as_buffer
+  | OID_BASIC_CONSTRAINTS        -> oid_BASIC_CONSTRAINTS_as_buffer
+  | OID_DIGEST_SHA224            -> oid_DIGEST_ALG_SHA224_as_buffer
+  | OID_DIGEST_SHA256            -> oid_DIGEST_ALG_SHA256_as_buffer
+  | OID_DIGEST_SHA384            -> oid_DIGEST_ALG_SHA384_as_buffer
+  | OID_DIGEST_SHA512            -> oid_DIGEST_ALG_SHA512_as_buffer
+
+let len_of_oid_buffer
+  (oid: oid_t)
+: Tot (len: asn1_value_int32_of_type OID
+      { v len == B.length (oid_buffer_of_oid oid) })
+      // { v len == Seq.length (normalize_term (oid_seq_of oid)) })
+= match oid with
+  | OID_DIGEST_SHA224 -> 9ul
+  | OID_DIGEST_SHA256 -> 9ul
+  | OID_DIGEST_SHA384 -> 9ul
+  | OID_DIGEST_SHA512 -> 9ul
+  | _ -> admit()
+
+noextract
+let seq_of_oid_buffer
+  (oid: oid_t)
+: Tot (s: bytes {List.mem s known_oids_as_seq /\
+                 B.witnessed (oid_buffer_of_oid oid) (IB.cpred s)})
+= oid_seq_of oid
+
+(*)
+inline_for_extraction
+let blit_from_ib
+  (src_seq: G.erased bytes) (* How to erase it? *)
+  (src: IB.ibuffer byte {B.frameOf src == HS.root /\ B.recallable src})
+  (src_from src_to: size_t)
+  (#rrel #rel: _)
+  (dst: B.mbuffer byte rrel rel)
+  (dst_pos: size_t)
+: HST.Stack unit
+  (requires (fun h ->
+    B.live h dst /\
+    v src_from <= v src_to /\ v src_to <= B.length src /\
+    v dst_pos + (v src_to - v src_from) <= B.length dst /\
+    // U32.v src_from <= U32.v src_to /\ U32.v src_to <= BY.length src /\
+    // U32.v dst_pos + (U32.v src_to - U32.v src_from) <= B.length dst /\
+    writable dst (v dst_pos) (v dst_pos + (v src_to - v src_from)) h
+  ))
+  (ensures (fun h _ h' ->
+    B.modifies (B.loc_buffer_from_to dst dst_pos (dst_pos + (src_to - src_from))) h h' /\
+    Seq.slice (B.as_seq h' dst) (v dst_pos) (v dst_pos + (v src_to - v src_from)) == Seq.slice (B.as_seq h src) (v src_from) (v src_to)
+  ))
+= let h0 = HST.get () in
+  HST.push_frame ();
+  let h1 = HST.get () in
+  let bi: B.pointer size_t = B.alloca 0ul 1ul in
+  let h2 = HST.get () in
+  let len = src_to - src_from in
+  C.Loops.do_while
+    (fun h stop ->
+      B.modifies (B.loc_union (B.loc_region_only true (HS.get_tip h1)) (B.loc_buffer_from_to dst dst_pos (dst_pos + len))) h2 h /\
+      B.live h bi /\ (
+      let i = Seq.index (B.as_seq h bi) 0 in
+      v i <= v len /\
+      writable dst (v dst_pos) (v dst_pos + v len) h /\
+      Seq.slice (B.as_seq h dst) (v dst_pos) (v dst_pos + v i) `Seq.equal` Seq.slice (B.as_seq h src) (v src_from) (v src_from + v i) /\
+      (stop == true ==> i == len)
+    ))
+    (fun _ ->
+      let i = B.index bi 0ul in
+      if i = len
+      then true
+      else begin
+        B.recall src;
+        IB.recall_value src src_seq;
+        let x = B.index src (src_from + i) in
+        mbuffer_upd dst (Ghost.hide (v dst_pos)) (Ghost.hide (v dst_pos + v len)) (dst_pos + i) x;
+        let i': size_t = i + 1ul in
+        B.upd bi 0ul i';
+        let h' = HST.get () in
+        Seq.lemma_split (Seq.slice (B.as_seq h' dst) (v dst_pos) (v dst_pos + v i')) (v i);
+        i' = len
+      end
+    )
+    ;
+  HST.pop_frame ()
+#pop-options
+*)
+
+#restart-solver
+#push-options "--query_stats --z3rlimit 16"
+inline_for_extraction
+let serialize32_asn1_oid_backwards
+  (len: asn1_value_int32_of_type OID)
+: Tot (serializer32_backwards (serialize_asn1_oid (v len)))
+= fun (oid: oid_t { Seq.length (oid_seq_of oid) == v len })
+    (#rrel #rel: _)
+    (b: B.mbuffer byte rrel rel)
+    (pos: size_t)
+-> (* Prf *) serialize_asn1_oid_unfold (v len) oid;
+   (* Prf *) serialize_asn1_oid_size (v len) oid;
+   let oid_buffer = oid_buffer_of_oid oid in
+   (* Prf *) B.recall oid_buffer;
+   (* Prf *) IB.recall_contents oid_buffer (seq_of_oid_buffer oid);
+
+   let offset = len_of_oid_buffer oid in
+
+   store_bytes
+     (* s32 *) (B32.of_buffer offset oid_buffer)
+     (*range*) 0ul offset
+     (* dst *) b
+     (* pos *) (pos - offset);
+
+(* return *) offset
+#pop-options
+
+   // (* Prf *) assert (
+   //   let s = B.as_seq h b in
+   //   let sub1:Seq.lseq byte 9 = Seq.create 9 0uy in
+   //   let sub2:Seq.lseq byte 9 = Seq.create 9 1uy in
+   //   let s1 = Seq.replace_subseq s (v pos - 9) (v pos) sub1 in
+   //   let s2 = Seq.replace_subseq s (v pos - 9) (v pos) sub2 in
+   //   Seq.lemma_index_create 9 0uy 0;
+   //   Seq.lemma_index_create 9 1uy 0;
+   //   s1.[v pos - 9] == 0uy /\
+   //   s2.[v pos - 9] == 1uy /\
+
+   //   (* diseq for seqs *)
+   //   sub1 =!= sub2 /\
+   //   ~ (s1 `Seq.equal` s2) /\
+
+   //   (* rel *)
+   //   s1 `rel` s2 /\
+   //   ~ (s1 `IB.immutable_preorder byte` s2) /\
+   //   ~ ( (s1 `rel` s2) <==> (s1 `IB.immutable_preorder byte` s2) ) /\
+   //   rel =!= (IB.immutable_preorder byte)
+   //   );
+
+   //   assert ( MB.rrel_rel_always_compatible rrel rel);
+
+open ASN1.Spec.Tag
+open ASN1.Spec.Length
+open ASN1.Low.Tag
+open ASN1.Low.Length
+
+inline_for_extraction
+let parser_tag_of_oid_impl
+  (x: datatype_of_asn1_type OID)
+: Tot (tg: (the_asn1_type OID & asn1_value_int32_of_type OID)
+      { tg == parser_tag_of_oid x })
+= (OID, len_of_oid_buffer x)
+
+#push-options "--query_stats --z3rlimit 32"
+inline_for_extraction
+let synth_asn1_oid_V_inverse_impl
+  (tg: (the_asn1_type OID & asn1_value_int32_of_type OID))
+  (value': refine_with_tag parser_tag_of_oid tg)
+: Tot (value: datatype_of_asn1_type OID
+      { length_of_oid value == v (snd tg) /\
+        value == synth_asn1_oid_V_inverse tg value' })
+= value'
+#pop-options
+
+let serialize32_asn1_oid_TLV_backwards ()
+: Tot (serializer32_backwards serialize_asn1_oid_TLV)
+= serialize32_tagged_union_backwards
+  (* lst *) (serialize32_asn1_tag_of_type_backwards OID
+             `serialize32_nondep_then_backwards`
+             serialize32_asn1_length_of_type_backwards OID)
+  (* tg  *) (parser_tag_of_oid_impl)
+  (* ls  *) (fun x -> (serialize32_synth_backwards
+                     (* ls1 *) (weak_kind_of_type OID
+                                `serialize32_weaken_backwards`
+                                serialize32_asn1_oid_backwards (snd x))
+                     (* f2  *) (synth_asn1_oid_V x)
+                     (* g1  *) (synth_asn1_oid_V_inverse x)
+                     (* g1' *) (synth_asn1_oid_V_inverse_impl x)
+                     (* Prf *) ()))
