src/asn1/ASN1.Low.Value.fst
@@ -5,4 +5,5 @@ include ASN1.Low.Value.NULL
 include ASN1.Low.Value.INTEGER
 include ASN1.Low.Value.OCTET_STRING
 include ASN1.Low.Value.BIT_STRING
+include ASN1.Low.Value.OID
 include ASN1.Low.Value.SEQUENCE
